coq-osiris/theories/semantics/micro.v
@@ -9,11 +9,12 @@ From osiris Require Import base.
 (* The monad is parameterized over a type constructor [code], which describes
    a set of services that a computation can request from the runtime system.
    These services can also be thought of as "system calls" that a computation
-   can make. A value of type [code X Y] represents the name of a system call
-   whose parameter has type [X] and whose result has type  [Y]. *)
+   can make. A value of type [code X Y E] represents the name of a system call
+   whose parameter has type [X], whose result has type [Y], and which can
+   throw an exception of type [E]. *)
 
 Module Type CODE.
-  Parameter code : Type → Type → Type.
+  Parameter code : Type → Type → Type → Type.
 End CODE.
 
 Module Make (C : CODE).
@@ -27,13 +28,13 @@ Import C. (* We write [code] for [C.code]. *)
    [return] and [bind] have their usual meaning.
 
    [try m f h] runs the computation [m]. If [m] returns a result [a] then the
-   computation [f a] is executed. If [m] ends with a soft failure [next], then
-   the computation [h()] is executed.
+   computation [f a] is executed. If [m] ends with an exception [throw e],
+   then the computation [h e] is executed.
 
    [crash] is a hard failure. It represents a crash and cannot be caught.
 
-   [next] is a soft failure. One can think of it as an exception. It can be
-   caught and handled using [try].
+   [throw e] causes a soft failure. One can think of it as an exception.
+   This exception can be caught and handled using [try].
 
    [stop c x] is a "system call", that is, a request for an external service.
    The code (i.e., the name) of the system call is [c] and its argument is
@@ -65,34 +66,34 @@ Import C. (* We write [code] for [C.code]. *)
    to a normal form. *)
 
 (* The constructor [Stop] is similar to the constructor [Vis] of interaction
-   trees. The type code is similar to an effect signature [E]. *)
+   trees. The type code is similar to an effect signature. *)
 
-Inductive micro A :=
+Inductive micro A E :=
   | Ret (a : A)
+  | Throw (e : E)
   | Crash
-  | Next
-  | Stop {X Y}
-      (c : code X Y) (x : X)
-      (k : Y → micro A)
-      (z : unit → micro A)
-  | Par {A1 A2}
-      (m1 : micro A1) (m2 : micro A2)
-      (k : A1 * A2 → micro A)
-      (z : unit → micro A)
-  | Choose {B}
-      (m1 m2 : micro B)
-      (k : B → micro A)
-      (z : unit → micro A)
+  | Stop {X Y E'}
+      (c : code X Y E') (x : X)
+      (k : Y → micro A E)
+      (z : E' → micro A E)
+  | Par {A1 A2 E'}
+      (m1 : micro A1 E') (m2 : micro A2 E')
+      (k : A1 * A2 → micro A E)
+      (z : E' → micro A E)
+  | Choose {B E'}
+      (m1 m2 : micro B E')
+      (k : B → micro A E)
+      (z : E' → micro A E)
 .
 
 (* Make [A] an implicit argument of the constructors. *)
 
-Arguments Ret    {A}.
-Arguments Crash  {A}.
-Arguments Next   {A}.
-Arguments Stop   {A X Y} c x k z.
-Arguments Par    {A A1 A2} m1 m2 k z.
-Arguments Choose {A B} m1 m2 k z.
+Arguments Ret    {A E}.
+Arguments Throw  {A E}.
+Arguments Crash  {A E}.
+Arguments Stop   {A E X Y E'} c x k z.
+Arguments Par    {A E A1 A2 E'} m1 m2 k z.
+Arguments Choose {A E B E'} m1 m2 k z.
 
 (* ------------------------------------------------------------------------ *)
 
@@ -101,34 +102,32 @@ Arguments Choose {A B} m1 m2 k z.
 Notation ret :=
   (Ret).
 
+Notation throw :=
+  (Throw).
+
 Notation crash :=
   (Crash).
-
-Notation next :=
-  (Next).
-
-Notation propagate :=
-  (λ tt, Next).
 
 (* [stop c x] stops, and, once restarted, behaves like the computation
    denoted by the code [c] applied to the argument [x]. The mapping of
    codes to computations is not defined here; it must be supplied a
    posteriori (step.v). *)
 
-Definition stop {X Y} (c : code X Y) x : micro Y :=
-  (Stop c x ret propagate).
+Definition stop {X Y E} (c : code X Y E) x : micro Y E :=
+  (Stop c x ret throw).
 
 (* [par m1 m2] runs the computations [m1] and [m2] in parallel,
    producing a pair of results. *)
 
-Definition par {A1 A2} (m1 : micro A1) (m2 : micro A2) : micro (A1 * A2) :=
-  Par m1 m2 ret propagate.
+Definition par {A1 A2 E} (m1 : micro A1 E) (m2 : micro A2 E)
+: micro (A1 * A2) E :=
+  Par m1 m2 ret throw.
 
 (* [choose m1 m2] performs a non-deterministic choice between [m1] and
    [m2] and runs the chosen computation, producing a single result. *)
 
-Definition choose {A} (m1 m2 : micro A) : micro A :=
-  Choose m1 m2 ret propagate.
+Definition choose {A E} (m1 m2 : micro A E) : micro A E :=
+  Choose m1 m2 ret throw.
 
 (* ------------------------------------------------------------------------ *)
 
@@ -140,16 +139,16 @@ Definition choose {A} (m1 m2 : micro A) : micro A :=
    [Stop], [Par], and [Choose]. So it is likely that this monad is not
    suitable for efficient executions of large computations inside Coq. *)
 
-Fixpoint bind {A B} (m : micro A) (f : A → micro B) : micro B :=
+Fixpoint bind {A B E} (m : micro A E) (f : A → micro B E) : micro B E :=
   match m with
   | Ret a =>
       f a
+  | Throw e =>
+      (* An exception is transmitted. *)
+      Throw e
   | Crash =>
       (* A hard failure is transmitted. *)
       Crash
-  | Next =>
-      (* A soft failure is transmitted. *)
-      Next
   | Stop c x k z =>
       (* A [Stop] effect is transmitted. The handler [bind _ f] remains
          installed on top of the continuations. *)
@@ -162,26 +161,21 @@ Fixpoint bind {A B} (m : micro A) (f : A → micro B) : micro B :=
       Choose m1 m2 (λ y, bind (k y) f) (λ y, bind (z y) f)
   end.
 
-Global Arguments bind A B !m f : simpl nomatch.
+Global Arguments bind A B E !m f : simpl nomatch.
 
 (* [try m f h] runs the computation [m]. If [m] returns a result [a] then the
-   computation [f a] is executed. If [m] ends with a soft failure [next] then
-   the computation [h()] is executed. *)
+   computation [f a] is executed. If [m] ends with an exception [throw e] then
+   the computation [h e] is executed. *)
 
-(* [h] must have type [unit → micro B], as opposed to just [micro B], because
-   we may wish to execute monadic computations (in Coq) using call-by-value
-   evaluation and we do not want to evaluate *both* branches in a [try]
-   construct. *)
-
-Fixpoint try {A B} (m : micro A) (f : A → micro B) (h : unit → micro B) : micro B :=
+Fixpoint try {A B E' E} (m : micro A E') (f : A → micro B E) (h : E' → micro B E) : micro B E :=
   match m with
   | Ret a =>
       f a
+  | Throw e =>
+      (* An exception is handled by [h]. *)
+      h e
   | Crash =>
       Crash
-  | Next =>
-      (* A soft failure is handled by [h]. *)
-      h()
   | Stop c x k z =>
       (* A [Stop] effect is transmitted. The handler [try _ f h] remains
          installed on top of the continuations. *)
@@ -200,9 +194,9 @@ Fixpoint try {A B} (m : micro A) (f : A → micro B) (h : unit → micro B) : mi
    definition of [bind] anyway, so as to prevent Coq from expanding uses
    of [bind] into more complex expressions that seem to involve [try]. *)
 
-Lemma bind_as_try {A B} (m : micro A) (f : A → micro B) :
+Lemma bind_as_try {A B E} (m : micro A E) (f : A → micro B E) :
   bind m f =
-  try m f propagate.
+  try m f throw.
 Proof.
   induction m; try solve [
     reflexivity
@@ -216,49 +210,54 @@ Global Hint Extern 1 (_ = _) => rewrite bind_as_try : bind_as_try.
 (* [orelse m1 m2] runs [m1] first. If [m1] succeeds, its result is
    transmitted. If [m1] fails, then [m2] is run. *)
 
-Definition orelse {A} (m1 m2 : micro A) : micro A :=
-  try m1 ret (λ tt, m2).
+Definition orelse {A E} (m1 m2 : micro A E) : micro A E :=
+  try m1 ret (λ _, m2).
 
 (* ------------------------------------------------------------------------ *)
 
 (* Paraphrase lemmas. *)
 
-Lemma bind_ret {A B} (a : A) (f : A → micro B) :
+(* TODO Some of these lemmas are unused. Remove them or make them Local. *)
+
+Lemma bind_ret {A B E} (a : A) (f : A → micro B E) :
   bind (ret a) f =
   f a.
 Proof.
   reflexivity.
 Qed.
 
-Lemma bind_crash {A B} (f : A → micro B) :
+Lemma bind_throw {A B E} (e : E) (f : A → micro B E) :
+  bind (throw e) f =
+  throw e.
+Proof.
+  reflexivity.
+Qed.
+
+Lemma bind_crash {A B E} (f : A → micro B E) :
   bind crash f =
   crash.
 Proof.
   reflexivity.
 Qed.
 
-Lemma bind_next {A B} (f : A → micro B) :
-  bind next f =
-  next.
-Proof.
-  reflexivity.
-Qed.
-
-Lemma bind_stop {A B X Y} (c : code X Y) x k z (f : A → micro B) :
+Lemma bind_stop {A B E X Y} (c : code X Y E) x k z (f : A → micro B E) :
   bind (Stop c x k z) f =
   Stop c x (λ y, bind (k y) f) (λ y, bind (z y) f).
 Proof.
   reflexivity.
 Qed.
 
-Lemma bind_par {A1 A2 A B} m1 m2 (k : A1 * A2 → micro A) z (f : A → micro B) :
+Lemma bind_par {A1 A2 A B E' E}
+  m1 m2 (k : A1 * A2 → micro A E) (z : E' → micro A E)
+  (f : A → micro B E) :
   bind (Par m1 m2 k z) f =
   Par m1 m2 (λ v, bind (k v) f) (λ y, bind (z y) f).
 Proof.
   reflexivity.
 Qed.
 
-Lemma bind_choose {A B C} m1 m2 (k : A → micro B) z (f : B → micro C) :
+Lemma bind_choose {A B C E' E}
+  m1 m2 (k : A → micro B E) (z : E' → micro B E) (f : B → micro C E) :
   bind (Choose m1 m2 k z) f =
   Choose m1 m2 (λ a, bind (k a) f) (λ a, bind (z a) f).
 Proof.
@@ -267,42 +266,45 @@ Qed.
 
 (* Analogous laws for [try]. *)
 
-Lemma try_ret {A B} (a : A) (f : A → micro B) (z : unit → micro B) :
+Lemma try_ret {A B E' E} (a : A) (f : A → micro B E) (z : E' → micro B E) :
   try (ret a) f z =
   f a.
 Proof.
   reflexivity.
 Qed.
 
-Lemma try_crash {A B} (f : A → micro B) (z : unit → micro B) :
+Lemma try_throw {A B E' E} (e : E') (f : A → micro B E) (z : E' → micro B E) :
+  try (throw e) f z =
+  z e.
+Proof.
+  reflexivity.
+Qed.
+
+Lemma try_crash {A B E' E} (f : A → micro B E) (z : E' → micro B E) :
   try crash f z =
   crash.
 Proof.
   reflexivity.
 Qed.
 
-Lemma try_next {A B} (f : A → micro B) (z : unit → micro B) :
-  try next f z =
-  z().
+Lemma try_Stop {A B E' E X Y}
+  (c : code X Y E') x k z (f : A → micro B E) (h : E' → micro B E) :
+  try (Stop c x k z) f h =
+  Stop c x (λ y, try (k y) f h) (λ y, try (z y) f h).
 Proof.
   reflexivity.
 Qed.
 
-Lemma try_Stop {A B X Y} (c : code X Y) x k z (f : A → micro B) z' :
-  try (Stop c x k z) f z' =
-  Stop c x (λ y, try (k y) f z') (λ y, try (z y) f z').
-Proof.
-  reflexivity.
-Qed.
-
-Lemma try_Par {A1 A2 A B} m1 m2 (k : A1 * A2 → micro A) z (f : A → micro B) z' :
+Lemma try_Par {A1 A2 A B E' E F}
+  m1 m2 (k : A1 * A2 → micro A E) (z : E' → micro A E)
+  (f : A → micro B F) (z' : E → micro B F) :
   try (Par m1 m2 k z) f z' =
   Par m1 m2 (λ v, try (k v) f z') (λ y, try (z y) f z').
 Proof.
   reflexivity.
 Qed.
 
-Lemma try_Choose {A B C} m1 m2 (k : A → micro B) z (k' : B → micro C) z' :
+Lemma try_Choose {A B C E' E F} m1 m2 (k : B → micro A E) (z : E' → micro A E) (k' : A → micro C F) (z' : E → micro C F) :
   try (Choose m1 m2 k z) k' z' =
   Choose m1 m2 (λ a, try (k a) k' z') (λ a, try (z a) k' z').
 Proof.
@@ -317,43 +319,37 @@ Global Hint Extern 1 (_ = _) => rewrite try_ret : try_ret.
 
 (* Equality is needed to state the monad laws. *)
 
-(* This equality is just equality of trees whose internal nodes are the
-   [Stop] nodes and whose leaves are [Ret], [Crash] and [Next]. *)
+(* This is just an equality of trees. *)
 
 (* We could give an inductive definition of this equality. I prefer to
    accept the law of functional extensionality, which implies that
    the desired equality coincides with Coq's ordinary equality. *)
 
-Lemma eq_stop_stop A X Y (k1 k2 : Y → micro A) (c : code X Y) x z1 z2 :
+Lemma eq_stop_stop {A E E' X Y} (c : code X Y E') x
+  (k1 k2 : Y → micro A E) (z1 z2 : E' → micro A E) :
   (∀ v, k1 v = k2 v) →
-  z1() = z2() →
+  (∀ e, z1 e = z2 e) →
   Stop c x k1 z1 = Stop c x k2 z2.
 Proof.
-  intros. f_equal.
-  { extensionality v. eauto. }
-  { extensionality tt. destruct tt. eauto. }
+  intros. f_equal; eauto using functional_extensionality.
 Qed.
 
-Lemma eq_par_par {A A1 A2} (m1 : micro A1) (m2 : micro A2)
-  (k k' : A1 * A2 → micro A) (z z' : unit → micro A) :
+Lemma eq_par_par {A A1 A2 E E'} m1 m2
+  (k k' : A1 * A2 → micro A E) (z z' : E' → micro A E) :
   (∀ v, k v = k' v) →
-  z() = z'() →
+  (∀ e, z e = z' e) →
   Par m1 m2 k z = Par m1 m2 k' z'.
 Proof.
-  intros. f_equal.
-  { extensionality v. eauto. }
-  { extensionality tt. destruct tt. eauto. }
+  intros. f_equal; eauto using functional_extensionality.
 Qed.
 
-Lemma eq_choose_choose {A B} (m1 : micro B) (m2 : micro B)
-  (k k' : B → micro A) (z z' : unit → micro A) :
+Lemma eq_choose_choose {A B E E'} m1 m2
+  (k k' : B → micro A E) (z z' : E' → micro A E) :
   (∀ v, k v = k' v) →
-  z() = z'() →
+  (∀ e, z e = z' e) →
   Choose m1 m2 k z = Choose m1 m2 k' z'.
 Proof.
-  intros. f_equal.
-  { extensionality v. eauto. }
-  { extensionality tt. destruct tt. eauto. }
+  intros. f_equal; eauto using functional_extensionality.
 Qed.
 
 Local Hint Resolve eq_stop_stop eq_par_par eq_choose_choose : eq.
@@ -365,47 +361,48 @@ Local Hint Resolve eq_stop_stop eq_par_par eq_choose_choose : eq.
 (* [bind_ret] has been proved already. *)
 
 Lemma bind_ret_right :
-  ∀ {A} (m : micro A),
+  ∀ {A E} (m : micro A E),
   bind m ret = m.
 Proof.
   induction m; simpl; eauto with eq.
 Qed.
 
 Lemma try_ret_right :
-  ∀ {A} (m : micro A),
-  try m ret propagate = m.
+  ∀ {A E} (m : micro A E),
+  try m ret throw = m.
 Proof.
   induction m; simpl; eauto with eq.
 Qed.
 
-Lemma bind_bind {A B C} (m : micro A) (f : A → micro B) (g : B → micro C) :
+Lemma bind_bind {A B C E} (m : micro A E) (f : A → micro B E) (g : B → micro C E) :
   bind (bind m f) g =
   bind m (λ a, bind (f a) g).
 Proof.
   induction m; simpl; eauto with eq.
 Qed.
 
-Lemma bind_try {A B C} (m : micro A) (f : A → micro B) (h : B → micro C) z :
+Lemma bind_try {A B C E E'}
+  m (f : A → micro B E) (z : E' → micro B E) (h : B → micro C E) :
   bind (try m f z) h =
   try m (λ a, bind (f a) h) (λ y, bind (z y) h).
 Proof.
   induction m; simpl; eauto with eq.
 Qed.
 
-Lemma try_bind {A B C} (m : micro A) (f : A → micro B) (k : B → micro C) z :
+Lemma try_bind {A B C E E'}
+  m (f : A → micro B E') (k : B → micro C E) (z : E' → micro C E) :
   try (bind m f) k z =
   try m (λ y, try (f y) k z) z.
 Proof.
   induction m; simpl; eauto with eq.
 Qed.
 
-Lemma try_try {A B C} (m : micro A) (f : A → micro B) (k : B → micro C) h z :
+Lemma try_try {A B C E E' E''} (m : micro A E'') (f : A → micro B E') (k : B → micro C E) h z :
   try (try m f h) k z =
   try m (λ y, try (f y) k z) (λ y, try (h y) k z).
 Proof.
   induction m; simpl; eauto with eq.
 Qed.
-
 
 Global Hint Extern 1 (_ = _) => rewrite bind_bind : bind_bind.
 Global Hint Extern 1 (_ = _) => rewrite bind_try : bind_try.
@@ -418,35 +415,35 @@ Global Hint Extern 1 (_ = _) => rewrite try_try : try_try.
    applications of [stop], [par], and [choose],
    wrapped in a [try] construct. *)
 
-Lemma try_stop {A X Y} c (x : X) (k : Y → micro A) z :
+Lemma try_stop {A X Y E E'} c (x : X) (k : Y → micro A E) (z : E' → micro A E) :
   try (stop c x) k z = Stop c x k z.
 Proof.
-  unfold stop. rewrite try_Stop. eauto using eq_stop_stop.
+  simpl try. eauto using eq_stop_stop.
 Qed.
 
-Lemma try_par {A1 A2 A} m1 m2 (k : A1 * A2 → micro A) z :
+Lemma try_par {A1 A2 A E E'} m1 m2 (k : A1 * A2 → micro A E) (z : E' → micro A E) :
   try (par m1 m2) k z = Par m1 m2 k z.
 Proof.
-  unfold par. rewrite try_Par. eauto using eq_par_par.
+  simpl try. eauto using eq_par_par.
 Qed.
 
-Lemma try_choose {A B} m1 m2 (k : A → micro B) z :
+Lemma try_choose {A B E E'} m1 m2 (k : A → micro B E) (z : E' → micro B E) :
   try (choose m1 m2) k z = Choose m1 m2 k z.
 Proof.
-  unfold choose. rewrite try_Choose. eauto using eq_choose_choose.
+  simpl try. eauto using eq_choose_choose.
 Qed.
 
 (* ------------------------------------------------------------------------ *)
 
 (* A 3-way case analysis principle: a computation [m] is either [ret a]
-   or [Next] or something else. *)
+   or [throw e] or something else. *)
 
-Lemma ret_or_next_or_else {A} (m : micro A) :
+Lemma ret_or_throw_or_else {A E} (m : micro A E) :
   (∃ a, m = ret a) ∨
-  (m = next) ∨
-  ((∀ a, m = ret a → False) ∧ (m = next → False)).
+  (∃ e, m = throw e) ∨
+  ((∀ a, m = ret a → False) ∧ (∀ e, m = throw e → False)).
 Proof.
-  destruct m; try solve [ eauto | right; right; split; congruence ].
+  destruct m; solve [ eauto | right; right; split; congruence ].
 Qed.
 
 (* ------------------------------------------------------------------------ *)
@@ -456,31 +453,32 @@ Qed.
    [try m _ _ = Par _ _ _ _]. They provide information about [m]. *)
 
 (* These lemmas are written in a form where one assumes that [m] is
-   not [ret _] or [Next]. This allows the conclusion to be simple.
+   not [ret _] or [throw _]. This allows the conclusion to be simple.
    Without this hypothesis, the conclusion of the lemma would have
    to be a 3-way disjunction. *)
 
-Lemma invert_try_eq_ret {A B m} {k : A → micro B} {z b} :
+Lemma invert_try_eq_ret {A B E E' m}
+  {k : A → micro B E} {z : E' → micro B E} {b} :
   try m k z = ret b →
   (∀ a, m = ret a → False) →
-  (m = next → False) →
+  (∀ e, m = throw e → False) →
   False.
 Proof.
-  destruct m; simpl; congruence.
+  destruct m; simpl; solve [ congruence | eauto ].
 Qed.
 
 Lemma invert_try_eq_stop
-  {A B m} {f : A → micro B} {h}
-  {X Y} {c : code X Y} {x k z} :
+  {A B E E' E'' m} {f : A → micro B E} {h : E' → micro B E}
+  {X Y} {c : code X Y E''} {x k z} :
   try m f h = Stop c x k z →
   (∀ a, m = ret a → False) →
-  (m = next → False) →
+  (∀ e, m = throw e → False) →
   ∃ k' z',
   m = Stop c x k' z' ∧
   k = (λ y, try (k' y) f h) ∧
   z = (λ y, try (z' y) f h).
 Proof.
-  destruct m; simpl; try congruence.
+  destruct m; simpl; try solve [ congruence | intros; exfalso; eauto ].
   intros H. dependent destruction H.
   intros _ _. eauto.
 Qed.
@@ -498,18 +496,19 @@ Ltac invert_try_eq_stop :=
       invert_try_eq_stop
   end.
 
-Lemma invert_try_eq_par {A A1 A2 B}
-  {m} {f : A → micro B} {h m1 m2} {k : A1 * A2 → micro B} {z}
+Lemma invert_try_eq_par {A A1 A2 B E E' E''}
+  {m : micro A E'} {f h}
+  {m1 m2} {k : A1 * A2 → micro B E} {z : E'' → micro B E}
 :
   try m f h = Par m1 m2 k z →
   (∀ a, m = ret a → False) →
-  (m = next → False) →
+  (∀ e, m = throw e → False) →
   ∃ k' z',
   m = Par m1 m2 k' z' ∧
   k = (λ y, try (k' y) f h) ∧
   z = (λ y, try (z' y) f h).
 Proof.
-  destruct m; simpl; try congruence.
+  destruct m; simpl; try solve [ congruence | intros; exfalso; eauto ].
   intros H. dependent destruction H.
   intros _ _. eauto.
 Qed.
@@ -527,18 +526,18 @@ Ltac invert_try_eq_par :=
       invert_try_eq_par
   end.
 
-Lemma invert_try_eq_choose {A B C}
-  {m} {f : A → micro B} {h m1 m2} {k : C → micro B} {z}
+Lemma invert_try_eq_choose {A B C E E' E''}
+  {m : micro A E'} {f h m1 m2} {k : C → micro B E} {z : E'' → micro B E}
 :
   try m f h = Choose m1 m2 k z →
   (∀ a, m = ret a → False) →
-  (m = next → False) →
+  (∀ e, m = throw e → False) →
   ∃ k' z',
   m = Choose m1 m2 k' z' ∧
   k = (λ y, try (k' y) f h) ∧
   z = (λ y, try (z' y) f h).
 Proof.
-  destruct m; simpl; try congruence.
+  destruct m; simpl; try solve [ congruence | intros; exfalso; eauto ].
   intros H. dependent destruction H.
   intros _ _. eauto.
 Qed.
