coq-osiris/theories/program_logic/helpers.v
@@ -24,13 +24,13 @@ Ltac wp_unfold m :=
 
 Section boilerplate.
 
-Context {A : Type}.
+Context {A X : Type}.
 Context `{!osirisGS Σ}.
 Implicit Type s : stuckness.
 Implicit Type P : iProp Σ.
 Implicit Type φ : A → iProp Σ.
 Implicit Type a : A.
-Implicit Type m : micro A.
+Implicit Type m : micro A X.
 
 (* [fupd_wp] states that to prove a WP behind a modality is enough to prove the
    WP without modality. This is particularly useful when using invariants. *)
@@ -185,7 +185,7 @@ Context `{!osirisGS Σ}.
 (* This technical lemma allows grabbing the state invariant when the
    goal is a [WP] assertion. *)
 
-Lemma wp_grab {A} (m : micro A) s E φ :
+Lemma wp_grab {A X} (m : micro A X) s E φ :
   (∀ σ, state_interp σ -∗
         |={E,∅}=> |={∅,E}=> state_interp σ ∗ WP m @ s; E {{ φ }}
   ) -∗
@@ -203,7 +203,7 @@ Qed.
 
 (* The assertion [WP m @ s; E {{ φ }}] is preserved by a reduction step. *)
 
-Lemma wp_step {A σ σ'} {m m' : micro A} {s E φ} :
+Lemma wp_step {A X σ σ'} {m m' : micro A X} {s E φ} :
   step (σ, m) (σ', m') →
   state_interp σ -∗
   WP m @ s; E {{ φ }} ={E,∅}=∗
@@ -223,13 +223,13 @@ Qed.
 
 (* [wp_preservation] is an iterated version of [wp_step]. *)
 Lemma wp_preservation n :
-  forall {A σ1 σn} {m1 mn : micro A} {s E φ},
+  forall {A X σ1 σn} {m1 mn : micro A X} {s E φ},
   nsteps step n (σ1, m1) (σn, mn) →
   state_interp σ1 -∗
   wp s E m1 φ ={E,∅}=∗
   |={∅}▷=>^n |={∅,E}=> state_interp σn ∗ wp s E mn φ.
 Proof.
-  induction n as [ | n IHn] => A σ1 σn m1 mn s E φ /=.
+  induction n as [ | n IHn] => A X σ1 σn m1 mn s E φ /=.
   { iIntros ([->->]%invert_nsteps_0%pair_equal_spec) "$$".
     iApply fupd_mask_subseteq; by apply empty_subseteq. }
   { iIntros (([σm mm]&Hstep&Hsteps)%nsteps_S_inv) "??".
@@ -241,7 +241,7 @@ Proof.
     { apply invert_nsteps_0 in Hsteps.
       simplify_eq/=. done. }
     { simpl. iMod "H" as "[??]".
-      iPoseProof (IHn _ _ _ _ _ _ _ _ Hsteps) as "IH".
+      iPoseProof (IHn _ _ _ _ _ _ _ _ _ Hsteps) as "IH".
       by iMod ("IH" with "[$][$]"). } }
 Qed.
 
@@ -251,7 +251,7 @@ Opaque stuck. (* TODO *)
 
 (* [wp_not_stuck] states that: The "Weakest Precondition" ensures the progress
    of computations.  *)
-Lemma wp_not_stuck {A} {σ} {m : micro A} s E {φ} :
+Lemma wp_not_stuck {A X} {σ} {m : micro A X} s E {φ} :
   state_interp σ -∗
   WP m @ s; E {{ φ }} -∗
   |={E,∅}=> ⌜ ¬ stuck (σ, m) ⌝.
@@ -272,7 +272,7 @@ Qed.
    imply that the machine configuration [(σ, m)] either can take a step
    or is finished. *)
 
-Lemma wp_can_step {A σ φ} {m: micro A} {s E}:
+Lemma wp_can_step {A X σ φ} {m: micro A X} {s E}:
   state_interp σ -∗
   wp s E m φ ={E,∅}=∗
   ⌜can_step (σ, m) ∨ is_ret m <> None ⌝.
@@ -289,7 +289,7 @@ Qed.
 
 (* Ditto, with a different mask. *)
 
-Lemma wp_can_step' {A σ φ} {m: micro A} {s E}:
+Lemma wp_can_step' {A X σ φ} {m: micro A X} {s E}:
   state_interp σ -∗
   wp s E m φ ={E}=∗
   ⌜can_step (σ, m) ∨ is_ret m <> None ⌝.
